backup before trying another way

Examples/MemSpec.v
@@ -19,10 +19,10 @@ Arguments MemSig : clear implicits.
 
 Module WriteRacyMem.
   Variant MemState {T V} :=
-  | MsIdle (heap : @Heap V)
-  | MsAllocPend (t : Name T) (heap : @Heap V)
-  | MsReadPend (t : Name T) (heap : @Heap V) (addr : Addr)
-  | MsWritePend (t : Name T) (heap : @Heap V) (addr : Addr) (val : V)
+  | MsIdle (heap : @Heap V) (loc : @Heap (Name T))
+  | MsAllocPend (t : Name T) (heap : @Heap V) (loc : @Heap (Name T))
+  | MsReadPend (t : Name T) (heap : @Heap V) (loc : @Heap (Name T)) (addr : Addr)
+  | MsWritePend (t : Name T) (heap : @Heap V) (loc : @Heap (Name T)) (addr : Addr) (val : V)
   | MsUBIdle
   | MsUBPend (t : Name T) {R : Type} (m : MemSig V R)
   | MsUBWritePend (t : Name T) {R : Type} (m : MemSig V R)
@@ -31,53 +31,60 @@ Module WriteRacyMem.
 
   Definition eval_heap {T V} (st : MemState T V) : option (@Heap V) :=
     match st with
-    | MsIdle h | MsAllocPend _ h | MsReadPend _ h _ | MsWritePend _ h _ _ => Some h
+    | MsIdle h _ | MsAllocPend _ h _ | MsReadPend _ h _ _ | MsWritePend _ h _ _ _ => Some h
     | _ => None
     end.
+  
+  Definition eval_loc  {T V} (st : MemState T V) : option (@Heap (Name T)) :=
+    match st with
+    | MsIdle _ loc | MsAllocPend _ _ loc | MsReadPend _ _ loc _ | MsWritePend _ _ loc _ _ => Some loc
+    | _ => None
+    end.
+  
 
   Variant MemStep {T V} : MemState T V -> (ThreadEvent T (MemSig V)) -> MemState T V -> Prop :=
     (* alloc steps *)
-    | MemMAllocCall i h:
-      MemStep (MsIdle h) (i, CallEv MAlloc) (MsAllocPend i h)
-    | MemMAllocRet i h (v:V) (l:Addr):
+    | MemMAllocCall i h loc:
+      MemStep (MsIdle h loc) (i, CallEv MAlloc) (MsAllocPend i h loc)
+    | MemMAllocRet i h loc (v:V) (l:Addr):
       (* allocate a new location *)
       h l = None ->
-      MemStep (MsAllocPend i h)
+      MemStep (MsAllocPend i h loc)
               (i, RetEv MAlloc l) 
               (* instantiate the location with some arbitrary value *)
-              (MsIdle (heap_update l v h))
+              (MsIdle (heap_update l v h) (heap_update l i loc))
     (* read steps *)
-    | MemReadCall i h l:
-      MemStep (MsIdle h) (i, CallEv (MRead l)) (MsReadPend i h l)
-    | MemReadRet i h l v:
+    | MemReadCall i h l loc:
+      MemStep (MsIdle h loc) (i, CallEv (MRead l)) (MsReadPend i h loc l)
+    | MemReadRet i h l v loc:
       (* can only read locations that are ready *)
       (* read pending values is undefined because the spec needs to ensure this will never happen *)
       h l = Some v ->
-      MemStep (MsReadPend i h l) (i, RetEv (MRead l) v) (MsIdle h)
-    | MemReadUndefined i h l v:
+      MemStep (MsReadPend i h loc l) (i, RetEv (MRead l) v) (MsIdle h loc)
+    | MemReadUndefined i h l v loc:
       (* read undefined locations cause UB *)
       h l = None ->
       (* read value is random *)
-      MemStep (MsReadPend i h l) (i, RetEv (MRead l) v) MsUBIdle
+      MemStep (MsReadPend i h loc l) (i, RetEv (MRead l) v) MsUBIdle
     (* write steps *)
-    | MemWriteCall i h l v:
-      MemStep (MsIdle h)
+    | MemWriteCall i h l v loc:
+      MemStep (MsIdle h loc)
               (i, CallEv (MWrite l v))
-              (MsWritePend i h l v)
-    | MemWriteCallRace i h l v j v':
+              (MsWritePend i h loc l v)
+    | MemWriteCallRace i h l v j v' loc:
       i <> j ->
-      MemStep (MsWritePend j h l v')
+      MemStep (MsWritePend j h loc l v')
               (i, CallEv (MWrite l v))
               (MsUBWritePend j (MWrite l v') i (MWrite l v))
-    | MemWriteRetUndef i h l v:
+    | MemWriteRetUndef i h l v loc:
       h l = None ->
-      MemStep (MsWritePend i h l v) (i, RetEv (MWrite l v) tt) MsUBIdle
-    | MemWriteRet i h l v v':
+      MemStep (MsWritePend i h loc l v) (i, RetEv (MWrite l v) tt) MsUBIdle
+    | MemWriteRet i h l v v' loc:
       h l = Some v' ->
-      MemStep (MsWritePend i h l v)
+      MemStep (MsWritePend i h loc l v)
               (i, RetEv (MWrite l v) tt)
               (* update the location to ready value after return *)
-              (MsIdle (heap_update l v h))
+              (MsIdle (heap_update l v h) loc)
     (* UB steps *)
     | MemStepUBCall i R (m : MemSig _ R):
       MemStep MsUBIdle (i, CallEv m) (MsUBPend i m)
@@ -90,12 +97,12 @@ Module WriteRacyMem.
 
   Definition mst2tst {T V} (st : MemState T V) (i : Name T) : option {R : Type & MemSig V R} :=
     match st with
-    | MsIdle _ | MsUBIdle => None
-    | MsAllocPend j _ =>
+    | MsIdle _ _ | MsUBIdle => None
+    | MsAllocPend j _ _ =>
         if i =? j then Some (existT _ _ MAlloc) else None
-    | MsReadPend j _ l =>
+    | MsReadPend j _ _ l =>
         if i =? j then Some (existT _ _ (MRead l)) else None
-    | MsWritePend j _ l v =>
+    | MsWritePend j _ _ l v =>
         if i =? j then Some (existT _ _ (MWrite l v)) else None
     | MsUBPend j m => 
         if i =? j then Some (existT _ _ m) else None
@@ -108,11 +115,11 @@ Module WriteRacyMem.
   Program Definition memSpec {T A} : Spec T (MemSig A) := {|
     State := MemState T A;
     Step := MemStep T A;
-    Init := MsIdle empty_heap
+    Init := MsIdle empty_heap empty_heap
   |}.
   Next Obligation.
     remember (fun _ : Name T => None) as tst.
-    remember (MsIdle empty_heap) as mst.
+    remember (MsIdle empty_heap empty_heap) as mst.
     assert (tst = mst2tst mst);
     [apply functional_extensionality; intros; subst; auto|].
     rewrite H0.
