Examples/WaitFreeStack.v
@@ -15,7 +15,8 @@ From LHL.Core Require Import
 From LHL.Util Require Import
   TransUtil
   Tactics
-  Util.
+  Util
+  Heap.
 
 From LHL.Examples Require Import
   CASSpec
@@ -37,6 +38,8 @@ Definition E A :=
   CASSig (Addr) |+| MemSig (A * option Addr).
 
 Definition F A := WaitFreeStackSig A.
+
+Axiom StkRet_inj : forall A B, StkRet A = StkRet B -> A = B.
 
 Definition wfpush {A} (v : A) : Prog (E A) (StkRet unit) :=
   old <- call Get;
@@ -80,22 +83,28 @@ Module AtomicWFStackProof.
   Notation casEv e := (inl e).
   Notation memEv e := (inr e).
 
-  Inductive list_seg (s:option Heap) : option Addr (*head*) -> option Addr (*tail*) -> list A (*list value*) -> Prop :=
-  | ListSegNil l h :
-      s = Some h ->
-      list_seg s l l nil
-  | ListSegCons h l l1 l2 l3 v vs:
-      l1 = Some l ->
-      s = Some h ->
-      h l = Some (v, l2) ->
-      list_seg s l2 l3 vs ->
-      list_seg s l1 l3 (v :: vs)
-  .
-  
-  Definition eval_stack_und (s:ISt) (vs : list A) : Prop :=
-    list_seg (eval_heap (memSt s)) (eval_cas (casSt s)) None vs.
-  
-  Section EvalStackLemma.
+  Section EvalStack.
+    Inductive list_seg (s:option Heap) : option Addr (*head*) -> option Addr (*tail*) -> list A (*list value*) -> Prop :=
+    | ListSegNil l h :
+        s = Some h ->
+        list_seg s l l nil
+    | ListSegCons h l l1 l2 l3 v vs:
+        l1 = Some l ->
+        s = Some h ->
+        h l = Some (v, l2) ->
+        list_seg s l2 l3 vs ->
+        list_seg s l1 l3 (v :: vs)
+    .
+
+    Definition eval_stack_und (s:ISt) (vs : list A) : Prop :=
+      list_seg (eval_heap (memSt s)) (eval_cas (casSt s)) None vs.
+    
+    Lemma ListSegSomeHeap: forall h l1 l2 vs,
+      list_seg h l1 l2 vs -> h <> None.
+    Proof.
+      destruct 1; congruence.
+    Qed.
+
     Lemma EvalStackSameUndState: forall (s1 s2:ISt) vs,
       snd s1 = snd s2 ->
       eval_stack_und s1 vs ->
@@ -107,7 +116,6 @@ Module AtomicWFStackProof.
       simpl. intros. subst. auto.
     Qed.
 
-    
     Lemma ListSegFrame: forall h l v hd tl vs,
       h l = None ->
       list_seg (Some h) hd tl vs ->
@@ -126,9 +134,87 @@ Module AtomicWFStackProof.
         + rewrite H0 in Heqs; inversion Heqs; subst.
           rewrite H1; auto.
     Qed.
-  End EvalStackLemma.
+
+    Lemma ListSegUnique: forall h hd tl vs1,
+      list_seg h hd tl vs1 ->
+      forall vs2, list_seg h hd tl vs2 ->
+      tl = None ->
+      vs1 = vs2.
+    Proof.
+      induction 1; intros; subst.
+      - inversion_clear H0; subst; auto.
+        congruence.
+      - inversion H3; subst.
+        inversion H0; subst.
+        inversion H; subst.
+        rewrite H1 in H4.
+        inversion H4; subst.
+        apply IHlist_seg in H5; subst; auto.
+    Qed.
+  End EvalStack.
+
+  Section OffChain.
+    Inductive off_chain_aux (s:option Heap) (l:Addr) : option Addr (*head*) -> option Addr (*tail*) -> Prop :=
+    | OffChainNil l1:
+      off_chain_aux s l l1 l1
+    | OffChainCons h l' l1 l2 l3 (v:A):
+        s = Some h ->
+        l1 = Some l' ->
+        h l' = Some (v, l2) ->
+        l <> l' ->
+        off_chain_aux s l l2 l3 ->
+        off_chain_aux s l l1 l3
+    .
+
+    Definition off_chain (s:ISt) (l:Addr) := off_chain_aux (eval_heap (memSt s)) l (eval_cas (casSt s)) None.
+
+    Lemma OffChainFrame: forall h hd tl vs new v,
+      list_seg (Some h) hd tl vs ->
+      h new = None ->
+      off_chain_aux (Some (heap_update new v h)) new hd tl.
+    Proof.
+      intros.
+      remember (Some h) as sh.
+      generalize dependent h.
+      induction H; intros; subst; try constructor.
+      inversion Heqsh; subst; clear Heqsh.
+      assert (new <> l).
+      {
+        unfold not; intros; subst.
+        congruence.
+      }
+      eapply OffChainCons with (v:=v0); eauto.
+      rewrite HeapUpdateOther; auto.
+    Qed.
+      
+    Lemma ListSegUpdateOffChain: forall h l1 vs new data,
+      list_seg (Some h) l1 None vs ->
+      off_chain_aux (Some h) new l1 None ->
+      list_seg (Some (heap_update new data h)) l1 None vs.
+    Proof.
+      intros.
+      remember None as l2.
+      revert H Heql2.
+      induction 1; intros; subst.
+      - eapply ListSegNil with (h:=(heap_update new data h)); auto.
+      - inversion H0; subst.
+        inversion H; inversion H1; subst.
+        inversion H4; subst.
+        rewrite H2 in H5. inversion H5; subst.
+        eapply ListSegCons with (l2:=l0); eauto.
+        rewrite HeapUpdateOther; auto.
+    Qed.
+  End OffChain.
   
 
+  Definition location_allocated (s:ISt) (l:Addr) : Prop :=
+    exists heap, eval_heap (memSt s) = Some heap /\ heap l <> None.
+
+  Definition location_owned (i:Name T) (s:ISt) (l:Addr) : Prop :=
+    location_allocated s l /\
+    exists loc, eval_loc (memSt s) = Some loc /\ loc l = Some i.
+  
+  
   Notation IStep s i e t :=
     (InterStep (WFStack _) s (i, UEvent (Some e)) t).
 
@@ -158,35 +244,43 @@ Module AtomicWFStackProof.
       IStep s1 i (RetEv (memEv MAlloc) new) s2 ->
       WFSTran i s1 ρ s2 ρ
     (* write *)
-    | StkWriteCall i s1 ρ s2 new data:
+    | StkWriteCall i s1 ρ s2 new data
+      (H_owned: location_owned i s1 new):
       IStep s1 i (CallEv (memEv (MWrite new data))) s2 ->
       WFSTran i s1 ρ s2 ρ
-    | StkWriteRet i s1 ρ s2 new data:
+    | StkWriteRet i s1 ρ s2 new data
+      (H_alloc: location_allocated s1 new)
+      (H_off_chain: off_chain s1 new):
       IStep s1 i (RetEv (memEv (MWrite new data)) tt) s2 ->
       WFSTran i s1 ρ s2 ρ
     (* read *)
     | StkReadCall i s1 ρ s2 addr:
       IStep s1 i (CallEv (memEv (MRead addr))) s2 ->
       WFSTran i s1 ρ s2 ρ
-    | StkReadRet i s1 ρ s2 addr v:
+    | StkReadRet i s1 ρ s2 addr v
+      (H_alloc: location_allocated s1 addr):
       IStep s1 i (RetEv (memEv (MRead addr)) v) s2 ->
       WFSTran i s1 ρ s2 ρ
     (* cas *)
     | StkCASCall i s1 ρ s2 old new:
       IStep s1 i (CallEv (casEv (CAS old new))) s2 ->
       WFSTran i s1 ρ s2 ρ
-    | StkCASRetPushPass i s1 s2 ρ1 ρ2 old new v:
-      (* TODO: side condition: new points to (v, old) *)
-      IStep s1 i (RetEv (casEv (CAS old new)) true) s2 ->
+    | StkCASRetPushPass i s1 s2 ρ1 ρ2 old new v h
+      (* new points to (v, old) *)
+      (H_heap: eval_heap (memSt s1) = Some h)
+      (H_new: h new = Some (v, old)):
+      IStep s1 i (RetEv (casEv (CAS old (Some new))) true) s2 ->
       VisPossSteps ρ1 [(i, CallEv (WFPush v)); (i, RetEv (WFPush v) (PASS tt))] ρ2 ->
       WFSTran i s1 ρ1 s2 ρ2
     | StkCASRetPushFail i s1 s2 ρ1 ρ2 old new v:
       IStep s1 i (RetEv (casEv (CAS old new)) false) s2 ->
       VisPossSteps ρ1 [(i, CallEv (WFPush v)); (i, RetEv (WFPush v) FAIL)] ρ2 ->
       WFSTran i s1 ρ1 s2 ρ2
-    | StkCASRetPopPass i s1 s2 ρ1 ρ2 old new v:
-      (* TODO: side condition: old points to (v, new) *)
-      IStep s1 i (RetEv (casEv (CAS old new)) true) s2 ->
+    | StkCASRetPopPass i s1 s2 ρ1 ρ2 old new v h
+      (* side condition: old points to (v, new) *)
+      (H_heap: eval_heap (memSt s1) = Some h)
+      (H_new: h old = Some (v, new)):
+      IStep s1 i (RetEv (casEv (CAS (Some old) new)) true) s2 ->
       VisPossSteps ρ1 [(i, CallEv WFPop); (i, RetEv WFPop (PASS (Some v)))] ρ2 ->
       WFSTran i s1 ρ1 s2 ρ2
     | StkCASRetPopFail i s1 s2 ρ1 ρ2 old new:
@@ -200,19 +294,209 @@ Module AtomicWFStackProof.
   Definition Rely (i : Name T) : Relt :=
     SRTC (fun s x t y => exists j, i <> j /\ WFSTran j s x t y).
 
+  Definition wfs_idle (x : Poss VF) : Prop := exists vs, PState x = WFSsIdle vs.
+
   Record Inv (s : ISt) (x : Poss VF) := {
-    stack_consistent :
-      eval_stack_und s (eval_stack (PState x))
+    (* overlay stack matches underlay stack *)
+    same_stack:
+      eval_stack_und s (eval_stack (PState x));
+    always_atomic:
+      wfs_idle x;
+    (* only write to location allocated by self *)
+    write_excl:
+      forall j h loc l v, MsWritePend j h loc l v = memSt s ->
+        loc l = Some j
+    (* loc_heap_match:
+      exists heap loc,
+        eval_heap (memSt s) = Some heap /\
+        eval_loc (memSt s) = Some loc /\
+        forall l, heap l <> None <-> loc l <> None *)
   }.
 
   Record Ready (i : Name T) (s : ISt) (x : Poss VF) := {
     ready_inv : Inv s x;
   }.
 
+  Record ReadyWaiting (i : Name T) {R} (m : F A R)
+  (s : InterState (F A) VE) (x : Poss VF)
+  := {
+    wait_ready : Ready i s x;
+    ready_wait : Waiting i m x
+  }.
+
   Record ReadyDone (i : Name T) {R} (m : F A R) (r : R) (s : ISt) (x : Poss VF) := {
     done_ready : Ready i s x;
     ready_done : Done i m r x;
   }.
+
+  Ltac begin_stable :=
+    unfold Stable, stablePost, stableRelt, stablePrec, sub, subRelt, subPrec;
+    unfold SStable, stableSRelt, stableSPrec, ssub, subSRelt, subSPrec;
+    unfold ReltToPrec, LiftSPrec, LiftSRelt;
+    intros; psimpl.
+    
+
+  Ltac subst_ist s :=
+    unfold eval_stack_und, casSt, memSt in *;
+    try match goal with
+    | HRewrite : _ = LState (snd s) |- _ =>
+      (repeat match goal with
+      | H : context[LState (snd s)] |- _ => 
+        lazymatch H with
+        | HRewrite => fail
+        | _ => setoid_rewrite <- HRewrite in H
+        end
+      end;
+      try match goal with
+      | |- context[LState (snd s)] =>
+        setoid_rewrite <- HRewrite
+      end)
+    end;
+    try match goal with
+    | HRewrite : LState (snd s) = _ |- _ =>
+      (* let x:= constr:(LState (snd s)) in  *)
+      (repeat match goal with
+      | H : context[LState (snd s)] |- _ => 
+        lazymatch H with
+        | HRewrite => fail
+        | _ => setoid_rewrite HRewrite in H
+        end
+      end;
+      try match goal with
+      | |- context[LState (snd s)] =>
+        setoid_rewrite HRewrite
+      end)
+    end;
+    try match goal with
+    | HRewrite : _ = RState (snd s) |- _ =>
+      (repeat match goal with
+      | H : context[RState (snd s)] |- _ => 
+        lazymatch H with
+        | HRewrite => fail
+        | _ => setoid_rewrite <- HRewrite in H
+        end
+      end;
+      try match goal with
+      | |- context[RState (snd s)] =>
+        setoid_rewrite <- HRewrite
+      end)
+    end;
+    try match goal with
+    | HRewrite : RState (snd s) = _ |- _ =>
+      (repeat match goal with
+      | H : context[RState (snd s)] |- _ => 
+        lazymatch H with
+        | HRewrite => fail
+        | _ => setoid_rewrite HRewrite in H
+        end
+      end;
+      try match goal with
+      | |- context[RState (snd s)] =>
+        setoid_rewrite HRewrite
+      end)
+    end.
+
+    Ltac forward_istep_cas_aux s1 s2 :=
+      match goal with
+      | same_stack0 : eval_stack_und _ _ |- _ =>
+        subst_ist s1; subst_ist s2;
+        simpl in *
+      end.
+
+    Ltac forward_istep_cas :=
+      match goal with
+        | H : IStep ?s1 _ _ ?s2 |- _ =>
+          destruct H as [_ [H ?]]; psimpl;
+          inversion H; subst; clear H;
+          forward_istep_cas_aux s1 s2
+      end.
+
+    (* Ltac mem_rewrite s1 s2 :=
+      unfold eval_stack_und, casSt, memSt in *;
+      subst_ist s1 s2. *)
+      (* try match goal with
+        | Hs1 : _ = LState (snd s1) |- _ =>
+          setoid_rewrite <- Hs1 in same_stack0
+        | Hs1 : LState (snd s1) = _ |- _ =>
+          setoid_rewrite Hs1 in same_stack0 end;
+        try match goal with
+        | Hs1 : _ = RState (snd s1) |- _ =>
+          setoid_rewrite <- Hs1 in same_stack0
+        | Hs1 : RState (snd s1) = _ |- _ =>
+          setoid_rewrite Hs1 in same_stack0 end;
+        try match goal with
+        | Hs2R : _ = RState (snd s2) |- _ =>
+          setoid_rewrite <- Hs2R
+        | Hs2R : RState (snd s2) = _ |- _ =>
+          setoid_rewrite Hs2R end;
+        try match goal with
+        | Hs2L : _ = LState (snd s2) |- _ =>
+          setoid_rewrite <- Hs2L 
+        | Hs2L : LState (snd s2) = _ |- _ =>
+          setoid_rewrite Hs2L
+          end. *)
+
+    Ltac forward_istep_mem_aux s1 s2 :=
+      match goal with
+      | same_stack0 : eval_stack_und _ _ |- _ =>
+        subst_ist s1; subst_ist s2;
+        simpl in *; try (inversion same_stack0; congruence)
+      end.
+  
+    Ltac forward_istep_mem :=
+      match goal with
+      | H: IStep ?s1 _ _ ?s2 |- _ =>
+        destruct H as [_ [H ?]]; psimpl;
+        inversion H; subst; clear H;
+        forward_istep_mem_aux s1 s2
+      end.
+  
+      Ltac unfold_possteps :=
+        repeat match goal with
+        | H:VisPossSteps _ _ _ |- _ =>
+          inversion H; subst; clear H
+        end.
+  
+      Ltac forward_pstep p1 p2 :=
+        match goal with
+        | H : VisPossStep p1 _ p2 |- _ =>
+          inversion H; subst; clear H;
+          match goal with
+          | H1 : Step _ (PState p1) _ (PState p2) |- _ =>
+            inversion H1; subst; clear H1
+          end
+        end.
+      
+      Ltac simp_eqs :=
+        do 10 try (
+          lazymatch goal with
+          | [ H1 : ?y = ?x, H2 : ?z = ?x |- _ ] =>
+            rewrite <- H2 in H1 at 1;
+            ddestruct H1
+          | [ H1 : ?x = ?y, H2 : ?z = ?x |- _ ] =>
+            rewrite H1 in H2;
+            ddestruct H2
+          | [ H1 : ?x = ?y, H2 : ?y = ?z |- _ ] =>
+            rewrite H2 in H1 at 1;
+            ddestruct H1
+          | [ H1 : ?x = ?y, H2 : ?z = ?y |- _ ] =>
+            rewrite <- H2 in H1 at 1;
+            ddestruct H1
+          | [ H : existT ?F ?A ?x = existT ?F ?A ?y |- _ ] =>
+            ddestruct H
+          end
+        ).
+  
+    Ltac drecs :=
+      do 10 try (
+        match goal with
+        | [ H : Inv ?s ?x |- _ ] =>
+          destruct H
+        | [ H : Ready ?i ?s ?x |- _ ] =>
+          destruct H
+        end
+      ).
+  
 
   Section SideConditions.
     Lemma RelyReflexive:
@@ -349,7 +633,7 @@ Module AtomicWFStackProof.
       exists i. split. easy.
       apply StkReturn. easy.
     Qed.
-
+    
     Lemma InitialReady:
       forall (i : Name T) (A0 : Type) (_ : F A A0),
       @LiftSPrec T (E A) (F A) VE VF (Ready i)
@@ -359,19 +643,19 @@ Module AtomicWFStackProof.
       unfold LiftSPrec.
       intros. eexists.
       split. easy.
-      constructor.
+      constructor; constructor.
       {
-        constructor. simpl eval_stack.
         unfold eval_stack_und.
         simpl. eapply ListSegNil. eauto.
       }
+      {
+        unfold wfs_idle. simpl; eauto.
+      }
+      {
+        unfold memSt; simpl.
+        inversion 1.
+      }
     Qed.
-    
-    Ltac begin_stable :=
-      unfold Stable, stablePost, stableRelt, stablePrec, sub, subRelt, subPrec;
-      unfold SStable, stableSRelt, stableSPrec, ssub, subSRelt, subSPrec;
-      unfold ReltToPrec, LiftSPrec, LiftSRelt;
-      intros; psimpl.
 
     Lemma sing_elem {A} {P : A -> Prop} :
       forall x : A,
@@ -381,156 +665,168 @@ Module AtomicWFStackProof.
     intros. now rewrite <- H.
     Qed.
 
-    Ltac forward_istep_cas stack_consistent0 :=
-    match goal with
-      | H : IStep ?s1 _ _ ?s2 |- _ =>
-        destruct H as [_ [H ?]]; psimpl;
-        unfold eval_stack_und, casSt, memSt in *;
-        inversion H; subst; clear H;
-        match goal with
-        | Hs1 : _ = LState (snd s1),
-          Hs2R : _ = RState (snd s2),
-          Hs2L : _ = LState (snd s2) |- _ =>
-          setoid_rewrite <- Hs2R;
-          setoid_rewrite <- Hs2L;
-          setoid_rewrite <- Hs1 in stack_consistent0
-        end
-      end.
-
-    Ltac forward_pstep p1 p2 :=
-      match goal with
-      | H : VisPossStep p1 _ p2 |- _ =>
-        inversion H; subst; clear H;
-        match goal with
-        | H1 : Step _ (PState p1) _ (PState p2) |- _ =>
-          inversion H1; subst; clear H1
-        end
-      end.
-    
-    Ltac simp_eqs :=
-      do 10 try (
-        lazymatch goal with
-        | [ H1 : ?y = ?x, H2 : ?z = ?x |- _ ] =>
-          rewrite <- H2 in H1 at 1;
-          ddestruct H1
-        | [ H1 : ?x = ?y, H2 : ?z = ?x |- _ ] =>
-          rewrite H1 in H2;
-          ddestruct H2
-        | [ H1 : ?x = ?y, H2 : ?y = ?z |- _ ] =>
-          rewrite H2 in H1 at 1;
-          ddestruct H1
-        | [ H1 : ?x = ?y, H2 : ?z = ?y |- _ ] =>
-          rewrite <- H2 in H1 at 1;
-          ddestruct H1
-        | [ H : existT ?F ?A ?x = existT ?F ?A ?y |- _ ] =>
-          ddestruct H
-        end
-      ).
-
     Lemma InvStable: forall i (s1 s2:InterState (F A) VE) p1 p2,
-      Ready i s1 p1 ->
-      (exists j, i <> j /\ WFSTran j s1 p1 s2 p2) ->
-      Ready i s2 p2.
+      Inv s1 p1 ->
+      WFSTran i s1 p1 s2 p2 ->
+      Inv s2 p2.
     Proof.
       intros.
-      destruct H0 as [j [? ?]].
-      constructor; constructor.
-      inversion_clear H.
-      inversion_clear ready_inv0.
-      inversion H1; subst; clear H1;
-      (* irrelevant cas events *)
-      try (forward_istep_cas stack_consistent0; now auto).
-      (* invoke any *)
+      (* destruct H0 as [j [? ?]]. *)
+      constructor.
       {
-        unfold InvokeAny, TInvoke, TIdle in H.
-        psimpl. apply sing_elem in H3. psimpl.
-        rewrite H5.
-        eapply EvalStackSameUndState; eauto.
+        inversion_clear H.
+        (* inversion_clear ready_inv0. *)
+        inversion H0; subst; clear H0;
+        (* irrelevant cas events *)
+        try (forward_istep_cas; now auto);
+        try (forward_istep_mem; now auto).
+        (* invoke any *)
+        {
+          unfold InvokeAny, TInvoke, TIdle in H.
+          psimpl. apply sing_elem in H2. psimpl.
+          rewrite H4.
+          eapply EvalStackSameUndState; eauto.
+        }
+        (* return any *)
+        {
+          unfold ReturnAny, TReturn, mapRetPoss in H.
+          psimpl. apply sing_elem in H2. psimpl.
+          rewrite H9.
+          eapply EvalStackSameUndState; eauto.
+        }
+        (* fail pop *)
+        {
+          forward_istep_cas.
+          unfold_possteps.
+          forward_pstep p1 y.
+          setoid_rewrite <- H1 in same_stack0.
+          forward_pstep y p2;
+          simp_eqs; simpl in *; auto.
+        }
+        (* malloc ret *)
+        {
+          forward_istep_mem.
+          apply ListSegFrame; auto.
+        }
+        (* write call *)
+        {
+          (* use write_excl, prevent concurrent writes *)
+          destruct H_owned as [_ [? [? ?]]].
+          forward_istep_mem.
+          inversion H0; subst x; clear H0.
+          specialize (write_excl0 _ _ _ _ _ eq_refl).
+          congruence.
+        }
+        (* write ret *)
+        {
+          forward_istep_mem.
+          {
+            destruct H_alloc as [? [? ?]].
+            setoid_rewrite <- H4 in H.
+            inversion H; subst x. congruence.
+          }
+          {
+            unfold off_chain in H_off_chain.
+            subst_ist s1. simpl in *.
+            apply ListSegUpdateOffChain; auto.
+          }
+        }
+        (* read ret *)
+        {
+          forward_istep_mem.
+          destruct H_alloc as [? [? ?]].
+          setoid_rewrite <- H4 in H.
+          simpl in H. congruence.
+        }
+        (* cas push succ *)
+        {
+          unfold_possteps.
+          forward_pstep p1 y.
+          setoid_rewrite <- H1 in same_stack0.
+          ddestruct H2. ddestruct H13.
+          forward_pstep y p2; simpl in *; simp_eqs.
+          - apply StkRet_inj in H13; subst. ddestruct H5.
+          (* this is the right branch *)
+          - forward_istep_cas.
+            + econstructor; eauto.
+            + apply pair_equal_spec in H17 as [_ H].
+              ddestruct H.
+        }
+        (* cas push fail *)
+        {
+          unfold_possteps.
+          forward_pstep p1 y.
+          setoid_rewrite <- H1 in same_stack0.
+          ddestruct H2. ddestruct H13.
+          forward_pstep y p2; simpl in *; simp_eqs.
+          forward_istep_cas; auto.
+          apply pair_equal_spec in H24 as [_ H].
+          ddestruct H.
+        }
+        (* cas pop succ *)
+        {
+          unfold_possteps.
+          forward_pstep p1 y.
+          setoid_rewrite <- H1 in same_stack0.
+          ddestruct H2. ddestruct H13.
+          forward_pstep y p2; simpl in *; simp_eqs.
+          - apply StkRet_inj in H13; subst. ddestruct H5.
+          - forward_istep_cas.
+            + inversion same_stack0; subst.
+              inversion H13; subst.
+              setoid_rewrite H_heap in H14.
+              inversion H14; subst.
+              rewrite H_new in H18.
+              inversion H18; subst; auto.
+            + apply pair_equal_spec in H13 as [_ H].
+              ddestruct H.
+        }
+        (* cas pop fail *)
+        {
+          unfold_possteps.
+          forward_pstep p1 y.
+          setoid_rewrite <- H1 in same_stack0.
+          ddestruct H2. ddestruct H13.
+          forward_pstep y p2; simpl in *; simp_eqs.
+          forward_istep_cas; auto.
+          apply pair_equal_spec in H24 as [_ H].
+          ddestruct H.
+        }
       }
-      (* return any *)
       {
-        unfold ReturnAny, TReturn, mapRetPoss in H.
-        psimpl. apply sing_elem in H3. psimpl.
-        rewrite H10.
-        eapply EvalStackSameUndState; eauto.
-      }
-      (* fail pop *)
-      {
-        forward_istep_cas stack_consistent0.
-        inversion H2; subst; clear H2.
-        inversion H16; subst; clear H16.
-        inversion H19; subst; clear H19.
-        forward_pstep p1 y.
-        setoid_rewrite <- H2 in stack_consistent0.
-        forward_pstep y p2;
-        simp_eqs; simpl in *; auto.
-      }
-      (* malloc call *)
-      {
-        destruct H as [_ [H ?]]; psimpl;
-        unfold eval_stack_und, casSt, memSt in *;
-        inversion H; subst; clear H;
-        match goal with
-        | Hs1 : _ = RState (snd s1) |- _ =>
-          setoid_rewrite <- Hs1 in stack_consistent0
-        end; simpl in *;
-        [|inversion stack_consistent0; congruence].
-        setoid_rewrite <- H4.
-        setoid_rewrite <- H8.
-        auto.
-      }
-      (* malloc ret *)
-      {
-        destruct H as [_ [H ?]]; psimpl;
-        unfold eval_stack_und, casSt, memSt in *;
-        inversion H; subst; clear H;
-        match goal with
-        | Hs1 : _ = RState (snd s1) |- _ =>
-          setoid_rewrite <- Hs1 in stack_consistent0
-        end; simpl in *;
-        [|inversion stack_consistent0; congruence
-         |inversion stack_consistent0; congruence].
-        setoid_rewrite <- H4.
-        setoid_rewrite <- H9.
-        simpl in *.
-        apply ListSegFrame; auto.
+        inversion_clear H.
+        inversion H0; subst; clear H0.
+        admit.
       }
       {
-        destruct H as [_ [H ?]]; psimpl;
-        unfold eval_stack_und, casSt, memSt in *;
-        inversion H; subst; clear H.
-        - (*provable*)
-          admit.
-        - (*unprovable*)
-          (* different threads should not be able to write to the same location *)
-          (* TODO: add extra field in mem state to record TID that allocates each location, and ensure in the rely that each thread only write to the one it allocates *)
-          admit.
-        - (*provable*)
-          admit.
+        inversion_clear H.
+        inversion H0; subst; clear H0;
+        (* irrelevant cas events *)
+        try (forward_istep_cas; now auto);
+        try (forward_istep_mem; now auto).
+        (* invoke any *)
+        {
+          unfold InvokeAny, TInvoke, TIdle in H.
+          psimpl. psimpl. unfold memSt in *.
+          setoid_rewrite H1 in write_excl0. auto.
+        }
+        (* return any *)
+        {
+          unfold ReturnAny, TReturn, mapRetPoss in H.
+          psimpl. unfold memSt in *.
+          setoid_rewrite H1 in write_excl0. auto.
+        }
+        {
+          forward_istep_mem.
+          inversion_clear 1.
+          destruct H_owned as [_ [? [? ?]]].
+          setoid_rewrite <- H5 in H.
+          inversion_clear H. auto.
+        }
       }
+    Admitted.
 
-        2:{
-          
-          setoid_rewrite <- H6 in stack_consistent0.
-        match goal with
-        | H : IStep ?s1 _ _ ?s2 |- _ =>
-          destruct H as [_ [H ?]]; psimpl;
-          unfold eval_stack_und, casSt, memSt in *;
-          inversion H; subst; clear H
-        end.
-          match goal with
-          | Hs1 : _ = LState (snd s1),
-            Hs2R : _ = RState (snd s2),
-            Hs2L : _ = LState (snd s2) |- _ =>
-            setoid_rewrite <- Hs2R;
-            setoid_rewrite <- Hs2L;
-            setoid_rewrite <- Hs1 in stack_consistent0
-          end
-        end.
-      }
-
-
-    Lemma InitialStable:
+    Lemma ReadyStable:
       forall (i : Name T) (A0 : Type) (_ : F A A0),
       @Stable T (E A) (F A) VE VF (@Logic.Prec T (E A) (F A) VE VF)
         (@stablePrec T (E A) (F A) VE VF) (@LiftSRelt T (E A) (F A) VE VF (Rely i))
@@ -540,55 +836,1465 @@ Module AtomicWFStackProof.
       specialize (H0 x1 eq_refl). psimpl.
       eexists. split. easy.
       induction H0; auto; clear H0.
+      destruct H as [? [_ ?]].
       apply IHSRTC; clear IHSRTC.
-      clear - H H1.
-      constructor; constructor.
       inversion_clear H1.
-      inversion_clear ready_inv0.
-      
-
-      destruct H as [j [? ?]].
-
-          (* {
-            
-          }
-          {
-            
-          }
-          {
-            unfold sub, subRelt, LiftSRelt.
-            intros. psimpl.
-            assert (exists x, σ = eq x).
-            {
-              unfold ReturnAny in H0. psimpl.
-              eapply Return_pres_single.
-              exact H0.
-            }
-            psimpl.
-            eexists. split. easy.
-            econstructor. 2: constructor.
-            exists i. split. easy.
-            apply StkReturn. easy.
-          } *)
-
-
-    (* Lemma RelyReflective :
-    forall (i : Name T) (s : InterState (F A) VE) (ρ : PossSet VF), Rely i s ρ s ρ.
-    2/10
-    forall i : Name T, Rely i ->> Rely i ==> Rely i
-    3/10
-    forall i j : Name T, i <> j -> Guar i ==> Rely j
-    4/10
-    forall i j : Name T, i <> j -> InvokeAny (WFStack A) i ==> Rely j
-    5/10
-    forall i j : Name T, i <> j -> ReturnAny (WFStack A) i ==> Rely j
-    6/10
-    forall (i : Name T) (A0 : Type), F A A0 -> Ready i (allIdle, Init VE) (eq initPoss)
-    7/10
-    forall (i : Name T) (A0 : Type), F A A0 -> Stable (Rely i) (Ready i) *)
-
+      constructor.
+      eapply InvStable; eauto.
+    Qed.
   End SideConditions.
   
+    Lemma SRTC_stable {P : Prec} {R : Relt} :
+      (forall s x t y,
+        P s x ->
+        R s x t y ->
+        P t y) ->
+      forall s x t y,
+        P s x ->
+        SRTC R s x t y ->
+        P t y.
+    Proof.
+      intros. induction H1. easy.
+      eapply IHSRTC, H. exact H0. easy.
+    Qed.
+
+    Lemma WaitingStable (i j : Name T) {R} (m : F A R) (s t : InterState (F A) VE) (x y : Poss VF) :
+      i <> j ->
+      Waiting i m x ->
+      WFSTran j s x t y ->
+      Waiting i m y.
+    Proof.
+      intros.
+      inversion H1; subst; clear H1;
+      auto; inversion_clear H0;
+      try (unfold_possteps;
+          repeat match goal with
+          | Hdf: differ_pointwise _ _ _ |- _ =>
+            specialize (Hdf _ H)
+          end; now simp_eqs).
+      {
+        unfold InvokeAny, TInvoke, TIdle in *.
+        psimpl.
+        apply sing_elem in H3. psimpl.
+        repeat match goal with
+        | Hdf: differ_pointwise _ _ _ |- _ =>
+          specialize (Hdf _ H) end;
+        constructor;
+        simp_eqs;
+        match goal with
+        | H: ?x = _ |- ?x = _ =>
+          rewrite H
+        end; auto.
+      }
+      {
+        unfold ReturnAny, TReturn, Returned, mapRetPoss in *.
+        psimpl.
+        apply sing_elem in H3. psimpl.
+        repeat match goal with
+        | Hdf: differ_pointwise _ _ _ |- _ =>
+          specialize (Hdf _ H) end;
+        constructor;
+        simp_eqs;
+        match goal with
+        | H: ?x = _ |- ?x = _ =>
+          rewrite H
+        end; auto.
+      }
+    Qed.
+
+    Lemma ready_waiting_stable (i : Name T) {R} (m : F A R) :
+      SStable (Rely i) (ReadyWaiting i m).
+    Proof.
+      begin_stable.
+      eapply SRTC_stable.
+      2: exact H. 2: exact H0.
+      clear. intros.
+      destruct H.
+      constructor;
+      destruct H0 as [j [? ?]].
+      {
+        inversion_clear wait_ready0.
+        constructor. eapply InvStable; eauto.
+      }
+      {
+        eapply WaitingStable; eauto.
+      }
+    Qed.
+
+    Lemma push_old_listseg_stable (i : Name T) v old:
+      SStable (Rely i) (fun s x =>
+        ReadyWaiting i (WFPush v) s x /\
+        exists vs, list_seg (eval_heap (memSt s)) old None vs
+      ).
+    Proof.
+      begin_stable.
+      remember (fun s (ρ:Poss VF) => ReadyWaiting i (WFPush v) s ρ /\
+      (exists vs : list A, list_seg (eval_heap (memSt s)) old None vs)) as P.
+      replace (ReadyWaiting i (WFPush v) s ρ /\
+      (exists vs : list A, list_seg (eval_heap (memSt s)) old None vs))
+      with (P s ρ); [|subst; auto].
+      eapply SRTC_stable;
+      subst; eauto.
+      clear. intros; simpl in *.
+      destruct H0 as [j [? ?]].
+      destruct H.
+      split.
+      {
+        eapply ready_waiting_stable.
+        psplit; eauto.
+        econstructor; eauto.
+        constructor.
+      }
+      
+      inversion H1; subst; clear H1;
+      try (match goal with
+      | H : IStep _ ?s1 _ ?s2 |- _ =>
+        inversion H; subst; clear H;
+        try match goal with
+        | H1 : StateStep _ _ _ |- _ =>
+          inversion H1; psimpl
+        end;
+        subst_ist s1; subst_ist s2
+      end; eauto).
+      {
+        unfold InvokeAny, TInvoke, TIdle in *. psimpl.
+        apply sing_elem in H5. psimpl.
+        unfold memSt in *.
+        setoid_rewrite <- H4. eauto.
+      }
+      {
+        unfold ReturnAny, TReturn, Returned, mapRetPoss in *. psimpl.
+        apply sing_elem in H5. psimpl.
+        unfold memSt in *.
+        setoid_rewrite <- H4. eauto.
+      }
+      {
+        inversion H3; subst; clear H3;
+        subst_ist s; subst_ist t; eauto.
+      }
+      {
+        inversion H3; subst; clear H3;
+        subst_ist s; subst_ist t;
+        simpl in *; eauto.
+        eapply ListSegFrame in H2; eauto.
+      }
+      {
+        destruct H_owned as [[? ?] [? [? ?]]].
+        inversion H3; subst; clear H3;
+        subst_ist s; subst_ist t;
+        simpl in *; eauto.
+        destruct H as [[[?]] _].
+        eapply write_excl0 in H12.
+        inversion H10; subst.
+        congruence.
+      }
+      {
+        destruct H_alloc as [? [? ?]].
+        inversion H3; subst; clear H3;
+        subst_ist s; subst_ist t;
+        simpl in *; eauto; try congruence.
+        inversion H9; subst x0.
+
+        destruct H as [[[?]] _].
+        eapply write_excl0 in H1.
+        eapply ListSegUpdateOffChain in H2; eauto.
+        
+        congruence.
+      }
+      3:{
+        inversion H2.
+        2:{}
+        (* inversion_clear ready_inv0. *)
+        (* inversion H2; subst; clear H2; *)
+        (* irrelevant cas events *)
+        try (forward_istep_cas; now eauto);
+        try (forward_istep_mem; now eauto).
+
+        
+
+        inversion H3
+        .
+
+        destruct H2 as [_ [H2 ?]]; psimpl;
+        inversion H2; subst; clear H2;
+        forward_istep_mem_aux s1 s2.
+        forward_istep_mem.
+      }
+    Admitted.
+
+    Lemma stepCall {E E' A B} {m : E' A} {k : A -> Prog E B} `{SigCoercion E' E} : (x <- call m; k x) = Bind (coerceOp _ m) k.
+    Proof.
+      rewrite frobProgId at 1. cbn.
+      f_equal. extensionality x.
+      rewrite frobProgId at 1. simpl.
+      apply foldProg.
+    Qed.
+
+    Ltac begin_commit :=
+      unfold Commit, LiftSPrec; intros.
+
+    Lemma eq_inj {A} :
+      forall x y : A,
+      eq x = eq y ->
+      x = y.
+    intros. now rewrite H.
+    Qed.
+
+  Lemma PushCorrect: forall (i:Name T) (v:A),
+    @VerifyProg T (E A) (F A) VE VF (StkRet unit) i
+    (@LiftSRelt T (E A) (F A) VE VF (Rely i))
+    (@LiftSRelt T (E A) (F A) VE VF (Guar i))
+    (@ReltCompose T (E A) (F A) VE VF
+      (@prComp T (E A) (F A) VE VF
+        (@LiftSPrec T (E A) (F A) VE VF (Ready i))
+        (@TInvoke T (E A) (F A) VE VF (WFStack A) i  (StkRet unit) (@WFPush A v)))
+      (@LiftSRelt T (E A) (F A) VE VF (Rely i)))
+    (WFStack A (StkRet unit) (@WFPush A v))
+    (fun r _ _ => LiftSPrec (ReadyDone i (WFPush v) r)).
+  Proof.
+    intros.
+
+    eapply weakenPrec with (P:=fun _ _ => LiftSPrec (ReadyWaiting i (WFPush v))).
+    2:{
+      unfold sub, subRelt, LiftSPrec, LiftSRelt.
+      intros. psimpl.
+      assert (x0 = eq (invPoss i x1 (WFPush v))).
+      {
+        unfold TInvoke in H1. psimpl. unfold invPoss.
+        set_ext y. split; intros; psimpl.
+        {
+          destruct x0, y. cbn in *.
+          f_equal. easy.
+          extensionality j.
+          dec_eq_nats i j.
+          now rewrite eqb_id.
+          now rewrite eqb_nid, H8.
+          extensionality j.
+          dec_eq_nats i j.
+          now rewrite eqb_id.
+          now rewrite eqb_nid, H9.
+        }
+        {
+          exists x1. split. easy.
+          cbn. rewrite eqb_id.
+          repeat split; (easy || apply differ_pointwise_trivial).
+        }
+      }
+      subst. specialize (H0 _ eq_refl).
+      psimpl. exists x0. split. easy.
+      assert (ReadyWaiting i (WFPush v) x (invPoss i x1 (WFPush v))).
+      {
+        assert (snd s = snd x).
+        { unfold TInvoke in H1. now psimpl. }
+        drecs.
+        constructor.
+        {
+          constructor.
+          constructor; cbn;
+          unfold wfs_idle, eval_stack_und, memSt, casSt in *;
+          auto; try now setoid_rewrite <- H.
+        }
+        {
+          constructor; cbn;
+          now rewrite eqb_id.
+        }
+      }
+      {
+        apply ready_waiting_stable.
+        psplit. exact H. easy.
+      }
+    }
+    
+    cut (
+      forall P,
+      P ==> (fun _ _ => LiftSPrec (ReadyWaiting i (WFPush v))) ->
+        VerifyProg i (LiftSRelt (Rely i)) (LiftSRelt (Guar i))
+          P
+          (wfpush v)
+          (fun r _ _ => LiftSPrec (ReadyDone i (WFPush v) r))
+    ).
+    { intros. now apply H. }
+    cofix rec. intros P impH. unfold wfpush.
+
+    (* step get call *)
+    rewrite stepCall.
+    eapply SafeBind with
+      (QI:=fun _ _ => LiftSPrec (ReadyWaiting i (WFPush v)))
+      (QR:=fun r _ _ => LiftSPrec (fun s x =>
+          ReadyWaiting i (WFPush v) s x /\
+          exists vs, list_seg (eval_heap (memSt s)) r None vs
+        )).
+    (* stable QI *)
+    {
+      begin_stable.
+      specialize (H0 x1 eq_refl) as [? [? ?]].
+      eexists; split; eauto.
+      apply ready_waiting_stable.
+      psplit; eauto.
+    }
+    (* stable QR *)
+    {
+      begin_stable.
+      specialize (H0 x1 eq_refl) as [? [? ?]].
+      eexists; split; eauto.
+      split.
+      - apply ready_waiting_stable.
+        psplit; eauto.
+      - eapply push_old_listseg_stable.
+        psplit; eauto.
+    }
+    (* commit *)
+    {
+      clear rec. begin_commit.
+      psimpl. apply impH in H.
+      clear impH. psimpl.
+      unfold LiftSPrec in H. psimpl.
+      exists (eq x).
+      split; [repeat econstructor|].
+      split; [intros; subst; repeat econstructor|].
+      split.
+      {
+        exists x. split; auto.
+        destruct H7, wait_ready0, ready_inv0.
+        constructor; [repeat constructor|auto].
+        - inversion H2; subst.
+          now forward_istep_cas_aux s t.
+        - admit.
+        - now setoid_rewrite <- H6.
+      }
+      {
+        exists x. split. easy. apply eq_inj in H; subst.
+        eapply StkGetCall with (i:=i).
+        constructor; [|easy].
+        constructor; cbn. easy.
+        intros. now rewrite H0.
+      }
+    }
+
+    (* step get ret *)
+    clear impH. intro old. split.
+    {
+      clear rec. begin_commit.
+      exists ρs.
+      psimpl. psimpl.
+      split; [repeat econstructor|].
+      split; [econstructor; split; [eauto|constructor]|].
+      split.
+      {
+        exists x3. split; auto.
+        destruct H4, wait_ready0, ready_inv0.
+        split.
+        {
+          constructor; [repeat constructor|auto].
+          - inversion H2; subst.
+            now forward_istep_cas_aux s t.
+          - admit.
+          - now setoid_rewrite <- H7.
+        }
+        {
+          unfold eval_stack_und in same_stack0.
+          exists (eval_stack (PState x3)).
+          setoid_rewrite <- H7.
+          inversion H2; subst.
+          setoid_rewrite <- H8 in same_stack0.
+          psimpl. now ddestruct H10.
+        }
+      }
+      {
+        exists x3. split. easy. apply eq_inj in H8; subst.
+        eapply StkGetRetId with (i:=i).
+        constructor.
+        - constructor; simpl; eauto.
+          now apply differ_pointwise_comm.
+        - constructor; auto.
+      }
+    }
+
+    (* step malloc call *)
+    rewrite stepCall.
+    eapply SafeBind with
+      (QI:=fun _ _ => LiftSPrec (fun s x =>
+          ReadyWaiting i (WFPush v) s x /\
+          exists vs, list_seg (eval_heap (memSt s)) old None vs
+        ))
+      (QR:=fun new _ _ => LiftSPrec (fun s x =>
+          ReadyWaiting i (WFPush v) s x /\
+          location_owned i s new /\
+          off_chain_aux (eval_heap (memSt s)) new (eval_cas (casSt s)) None /\
+          off_chain_aux (eval_heap (memSt s)) new old None /\
+          exists vs, list_seg (eval_heap (memSt s)) old None vs
+        )).
+    (* QI stable *)
+    { admit. }
+    (* QR stable *)
+    { admit. }
+    (* commit *)
+    {
+      clear rec. begin_commit.
+      psimpl. psimpl.
+      exists (eq x5).
+      split; [repeat econstructor|].
+      split; [intros; subst; repeat econstructor|].
+      split.
+      {
+        exists x5. split; auto.
+        destruct H5, wait_ready0, ready_inv0.
+        split.
+        {
+          constructor; [repeat constructor|auto];
+          inversion H2; subst; forward_istep_mem_aux s t.
+        }
+        {
+          inversion H2; subst; forward_istep_mem_aux s t.
+          eexists; eauto.
+        }
+      }
+      {
+        exists x5. split. easy. apply eq_inj in H10; subst.
+        eapply StkAllocCall with (i:=i).
+        constructor; [|easy].
+        constructor; cbn. easy.
+        intros. now rewrite H0.
+      }
+    }
+
+    (* step malloc ret *)
+    intro new. split.
+    {
+      clear rec. begin_commit.
+      exists ρs.
+      psimpl. psimpl.
+      split; [repeat econstructor|].
+      split; [econstructor; split; [eauto|constructor]|].
+      split.
+      {
+        exists x4. split; auto.
+        destruct H4, wait_ready0, ready_inv0.
+        split; [|split; [split|split;[|split]]].
+        {
+          constructor; [repeat constructor|auto];
+          inversion H2; subst; forward_istep_mem_aux s t.
+          eapply ListSegFrame; eauto.
+        }
+        {
+          inversion H2; subst; forward_istep_mem_aux s t.
+          exists (heap_update l v0 h).
+          setoid_rewrite <- H15.
+          split; auto.
+          ddestruct H14.
+          rewrite HeapUpdateSelf; congruence.
+        }
+        {
+          unfold location_owned.
+          inversion H2; subst; forward_istep_mem_aux s t.
+          eexists; split; [reflexivity|].
+          ddestruct H14. apply HeapUpdateSelf.
+        }
+        {
+          inversion H2; subst; forward_istep_mem_aux s t.
+          ddestruct H14.
+          eapply OffChainFrame; eauto.
+        }
+        {
+          inversion H2; subst; forward_istep_mem_aux s t.
+          ddestruct H14.
+          eapply OffChainFrame; eauto.
+        }
+        {
+          inversion H2; subst; forward_istep_mem_aux s t.
+          eapply ListSegFrame in H5; eauto.
+        }
+      }
+      {
+        exists x4. split. easy. apply eq_inj in H12; subst.
+        eapply StkAllocRet with (i:=i).
+        constructor.
+        - constructor; simpl; eauto.
+          now apply differ_pointwise_comm.
+        - constructor; auto.
+      }
+    }
+
+    (* step write call *)
+    rewrite stepCall.
+    eapply SafeBind with
+      (QI:=fun _ _ => LiftSPrec (fun s x =>
+          ReadyWaiting i (WFPush v) s x /\
+          location_owned i s new /\
+          off_chain_aux (eval_heap (memSt s)) new (eval_cas (casSt s)) None /\
+          off_chain_aux (eval_heap (memSt s)) new old None /\
+          exists vs, list_seg (eval_heap (memSt s)) old None vs
+        ))
+      (QR:=fun _ _ _ => LiftSPrec (fun s x =>
+          ReadyWaiting i (WFPush v) s x /\
+          (exists h, (eval_heap (memSt s)) = Some h /\ h new = Some (v, old)) /\
+          exists vs, list_seg (eval_heap (memSt s)) old None vs
+          (* /\
+          list_seg (eval_heap (memSt s)) (Some new) None (v :: vs) *)
+        )).
+    (* QI stable *)
+    { admit. }
+    (* QR stable *)
+    { admit. }
+    (* commit *)
+    {
+      clear rec. begin_commit.
+      psimpl. psimpl.
+      exists (eq x6).
+      split; [repeat econstructor|].
+      split; [intros; subst; repeat econstructor|].
+      split.
+      {
+        exists x6. split; auto.
+        destruct H5, wait_ready0, ready_inv0.
+        inversion H2; subst; forward_istep_mem_aux s t.
+        {
+          split; [|split;[|split]]; auto.
+          {
+            constructor; [repeat constructor|auto];
+            subst_ist s; subst_ist t; auto.
+            inversion_clear 1.
+            destruct H6 as [_ [? [? ?]]].
+            subst_ist s.
+            now inversion_clear H5.
+          }
+          {
+            unfold location_owned in *.
+            destruct H6 as [? [? [? ?]]].
+            subst_ist s; subst_ist t.
+            inversion H6; subst x2.
+            split; eauto.
+            unfold location_allocated in *.
+            now subst_ist s; subst_ist t.
+          }
+          {
+            eexists; eauto.
+          }
+        }
+        {
+          exfalso.
+          unfold location_owned in *.
+          destruct H6 as [_ [? [? ?]]].
+          subst_ist s; subst_ist t.
+          inversion H6; subst x2.
+          specialize write_excl0 with (1:=eq_refl).
+          congruence.
+        }
+      }
+      {
+        exists x6. split. easy. apply eq_inj in H17; subst.
+        eapply StkWriteCall with (i:=i) (data:=(v,old)); [exact H6|].
+        constructor; [|easy].
+        constructor; cbn. easy.
+        intros. now rewrite H0.
+      }
+    }
+
+    (* step write ret *)
+    intros. destruct v0. split.
+    {
+      clear rec. begin_commit.
+      exists ρs.
+      psimpl. psimpl.
+      split; [repeat econstructor|].
+      split; [econstructor; split; [eauto|constructor]|].
+      split.
+      {
+        exists x4. split; auto.
+        destruct H4, wait_ready0, ready_inv0.
+        inversion H2; subst; forward_istep_mem_aux s t.
+        {
+          exfalso.
+          destruct H5 as [[? [? ?]] _].
+          setoid_rewrite <- H4 in H5.
+          simpl in H5. congruence.
+        }
+        split; [|split].
+        {
+          constructor; [repeat constructor|auto];
+          subst_ist s; subst_ist t; psimpl; auto.
+          - eapply ListSegUpdateOffChain; eauto.
+          - inversion 1.
+        }
+        {
+          eexists; split; eauto.
+          apply HeapUpdateSelf.
+        }
+        {
+          eapply ListSegUpdateOffChain in H7; eauto.
+        }
+      }
+      {
+        exists x4. split. easy. apply eq_inj in H19; subst.
+        eapply StkWriteRet with (i:=i) (data:=(v, old)); eauto.
+        - destruct H5 as [? _]. auto.
+        - constructor.
+          + constructor; simpl; eauto.
+            now apply differ_pointwise_comm.
+          + constructor; auto.
+      }
+    }
+
+    (* step cas call *)
+    rewrite stepCall.
+    eapply SafeBind with
+      (QI:=fun _ _ => LiftSPrec (fun s x =>
+          ReadyWaiting i (WFPush v) s x /\
+          (exists h, (eval_heap (memSt s)) = Some h /\ h new = Some (v, old)) /\
+          exists vs, list_seg (eval_heap (memSt s)) old None vs
+        ))
+      (QR:=fun r _ _ => 
+          if r : bool
+          then LiftSPrec (ReadyDone i (WFPush v) (PASS tt))
+          else LiftSPrec (ReadyDone i (WFPush v) FAIL)).
+    (* QI stable *)
+    { admit. }
+    (* QR stable *)
+    { admit. }
+    (* commit *)
+    {
+      clear rec. begin_commit.
+      psimpl. psimpl.
+      exists (eq x6).
+      split; [repeat econstructor|].
+      split; [intros; subst; repeat econstructor|].
+      split.
+      {
+        exists x6. split; auto.
+        destruct H5, wait_ready0, ready_inv0.
+        inversion H2; subst; forward_istep_cas_aux s t.
+        split; auto.
+        {
+          constructor; [repeat constructor|auto];
+          subst_ist s; subst_ist t; auto.
+        }
+        {
+          eexists; eauto.
+        }
+      }
+      {
+        exists x6. split. easy. apply eq_inj in H23; subst.
+        eapply StkCASCall with (i:=i) (old:=old) (new:=Some new).
+        constructor; [|easy].
+        constructor; cbn. easy.
+        now apply differ_pointwise_comm.
+      }
+    }
+
+    (* step cas ret *)
+    intros. split.
+    {
+      clear rec. begin_commit.
+      psimpl.
+      destruct H4, wait_ready0, ready_inv0.
+      destruct always_atomic0 as [vs ?].
+      destruct x4; simpl in *.
+      destruct ready_wait0.
+      psimpl. psimpl.
+      inversion H2; subst; forward_istep_cas_aux s t;
+      ddestruct H34; psimpl.
+      (* cas succ *)
+      {
+        exists (eq (
+          comRetPoss i
+            (comInvPoss i
+              (MkPoss T (F A) VF (WFSsIdle vs) PCalls PRets)
+              (WFPush v)
+              (WFSsPend i vs (WFPush v))
+            )
+            (WFPush v)
+            (WFSsIdle (v :: vs))
+            (PASS tt)
+        )).
+        split; [repeat econstructor|].
+        split; [econstructor; split; [now eauto|]|split].
+        (* poss step *)
+        {
+          subst.
+          (* commit call *)
+          eapply PossStepsStep with (i := i) (σ := (comInvPoss i
+            (MkPoss T (F A) VF (WFSsIdle vs) PCalls PRets)
+            (WFPush v)
+            (WFSsPend i vs (WFPush v))
+          )); psimpl; auto.
+          {
+             eapply PCommitCall with (m := WFPush v); psimpl; auto;
+             [constructor|now rewrite eqb_id].
+          }
+          {
+            intros; rewrite eqb_nid; auto.
+          }
+          (* commit ret *)
+          eapply PossStepsStep with (i := i);
+          [| | |apply PossStepsRefl];
+          psimpl; auto.
+          {
+            eapply PCommitRet with (m := WFPush v) (v := PASS tt);
+            psimpl; auto; try now rewrite eqb_id.
+            constructor.
+          }
+          {
+            intros; rewrite eqb_nid; auto.
+          }
+        }
+        (* post condition *)
+        {
+          assert (vs = x5) by (eapply ListSegUnique; eauto); subst x5.
+          eexists; split; eauto.
+          constructor; constructor; [constructor| |]; psimpl;
+          try now rewrite eqb_id.
+          - subst_ist s; subst_ist t; psimpl; auto.
+            econstructor; eauto.
+          - unfold wfs_idle in *; psimpl; eauto.
+          - subst_ist s; subst_ist t; auto.
+        }
+        (* guarantee *)
+        {
+          exists (comRetPoss i
+          (comInvPoss i (MkPoss T (F A) VF (WFSsIdle vs) PCalls PRets) 
+             (WFPush v) (WFSsPend i vs (WFPush v))) (WFPush v) (WFSsIdle (v :: vs)) 
+          (PASS tt)).
+          split. easy. apply eq_inj in H20; subst.
+          (* inversion H6; subst; clear H6. *)
+          eapply StkCASRetPushPass with (i:=i) (v:=v) (new:=new) (old:=old); eauto.
+          constructor.
+          - constructor; simpl; eauto.
+            now apply differ_pointwise_comm.
+          - constructor; psimpl; auto.
+            subst_ist s; subst_ist t; auto.
+          - eapply VStep with (y:=comInvPoss i
+              (MkPoss T (F A) VF (WFSsIdle vs) PCalls PRets)
+              (WFPush v)
+              (WFSsPend i vs (WFPush v))); psimpl; auto;
+              [
+                constructor; psimpl; auto;
+                [constructor|now rewrite eqb_id]|
+                apply differ_pointwise_trivial|
+                unfold differ_pointwise; auto|
+              ].
+            eapply VStep; [| | |apply VRefl];
+            psimpl; auto;
+            try apply differ_pointwise_trivial;
+            try (unfold differ_pointwise; auto).
+            constructor; psimpl; auto;
+            try now rewrite eqb_id.
+            constructor.
+        }
+      }
+      (* cas fail *)
+      {
+        exists (eq (
+          comRetPoss i
+            (comInvPoss i
+              (MkPoss T (F A) VF (WFSsIdle vs) PCalls PRets)
+              (WFPush v)
+              (WFSsPend i vs (WFPush v))
+            )
+            (WFPush v)
+            (WFSsIdle vs)
+            (FAIL)
+        )).
+        split; [repeat econstructor|].
+        split; [econstructor; split; [now eauto|]|split].
+        (* poss step *)
+        {
+          subst.
+          (* commit call *)
+          eapply PossStepsStep with (i := i) (σ := (comInvPoss i
+            (MkPoss T (F A) VF (WFSsIdle vs) PCalls PRets)
+            (WFPush v)
+            (WFSsPend i vs (WFPush v))
+          )); psimpl; auto.
+          {
+             eapply PCommitCall with (m := WFPush v); psimpl; auto;
+             [constructor|now rewrite eqb_id].
+          }
+          {
+            intros; rewrite eqb_nid; auto.
+          }
+          (* commit ret *)
+          eapply PossStepsStep with (i := i);
+          [| | |apply PossStepsRefl];
+          psimpl; auto.
+          {
+            eapply PCommitRet with (m := WFPush v) (v := FAIL);
+            psimpl; auto; try now rewrite eqb_id.
+            constructor.
+          }
+          {
+            intros; rewrite eqb_nid; auto.
+          }
+        }
+        (* post condition *)
+        {
+          eexists; split; eauto.
+          constructor; constructor; [constructor| |]; psimpl;
+          try (now rewrite eqb_id);
+          subst_ist s; subst_ist t; psimpl; auto.
+          unfold wfs_idle in *; psimpl; eauto.
+        }
+        (* guarantee *)
+        {
+          exists (comRetPoss i
+          (comInvPoss i (MkPoss T (F A) VF (WFSsIdle vs) PCalls PRets) 
+             (WFPush v) (WFSsPend i vs (WFPush v))) (WFPush v) 
+          (WFSsIdle vs) FAIL).
+          split. easy. apply eq_inj in H20; subst.
+          (* inversion H6; subst; clear H6. *)
+          eapply StkCASRetPushFail with (i:=i) (v:=v) (new:=Some new) (old:=old); eauto.
+          constructor.
+          - constructor; simpl; eauto.
+            now apply differ_pointwise_comm.
+          - constructor; psimpl; auto.
+            subst_ist s; subst_ist t; auto.
+          - eapply VStep with (y:=comInvPoss i
+              (MkPoss T (F A) VF (WFSsIdle vs) PCalls PRets)
+              (WFPush v)
+              (WFSsPend i vs (WFPush v))); psimpl; auto;
+              [
+                constructor; psimpl; auto;
+                [constructor|now rewrite eqb_id]|
+                apply differ_pointwise_trivial|
+                unfold differ_pointwise; auto|
+              ].
+            eapply VStep; [| | |apply VRefl];
+            psimpl; auto;
+            try apply differ_pointwise_trivial;
+            try (unfold differ_pointwise; auto).
+            constructor; psimpl; auto;
+            try now rewrite eqb_id.
+            constructor.
+        }
+      }
+    }
+
+    (* ret *)
+    destruct v0; psimpl.
+    {
+      apply SafeReturn.
+      unfold sub, subRelt.
+      intros. unfold LiftSPrec in H.
+      psimpl. exists x4. now destruct H3.
+    }
+    {
+      apply SafeReturn.
+      unfold sub, subRelt.
+      intros. unfold LiftSPrec in H.
+      psimpl. exists x4. now destruct H3.
+    }
+  Admitted.
+
+  Lemma PopCorrect: forall (i : Name T),
+    @VerifyProg T (E A) (F A) VE VF (StkRet (option A)) i
+      (@LiftSRelt T (E A) (F A) VE VF (Rely i))
+      (@LiftSRelt T (E A) (F A) VE VF (Guar i))
+      (@ReltCompose T (E A) (F A) VE VF
+        (@prComp T (E A) (F A) VE VF (@LiftSPrec T (E A) (F A) VE VF (Ready i))
+            (@TInvoke T (E A) (F A) VE VF (WFStack A) i (StkRet (option A)) (@WFPop A)))
+        (@LiftSRelt T (E A) (F A) VE VF (Rely i)))
+      (WFStack A (StkRet (option A)) (@WFPop A))
+      (fun (r : StkRet (option A)) (_ : @InterState T (E A) (F A) VE)
+        (_ : @PossSet T (F A) VF) =>
+      @LiftSPrec T (E A) (F A) VE VF (@ReadyDone i (StkRet (option A)) (@WFPop A) r)).
+  Proof.
+    intros.
+    eapply weakenPrec with (P:=fun _ _ => LiftSPrec (ReadyWaiting i WFPop)).
+    2:{
+      unfold sub, subRelt, LiftSPrec, LiftSRelt.
+      intros. psimpl.
+      assert (x0 = eq (invPoss i x1 WFPop)).
+      {
+        unfold TInvoke in H1. psimpl. unfold invPoss.
+        set_ext y. split; intros; psimpl.
+        {
+          destruct x0, y. cbn in *.
+          f_equal. easy.
+          extensionality j.
+          dec_eq_nats i j.
+          now rewrite eqb_id.
+          now rewrite eqb_nid, H8.
+          extensionality j.
+          dec_eq_nats i j.
+          now rewrite eqb_id.
+          now rewrite eqb_nid, H9.
+        }
+        {
+          exists x1. split. easy.
+          cbn. rewrite eqb_id.
+          repeat split; (easy || apply differ_pointwise_trivial).
+        }
+      }
+      subst. specialize (H0 _ eq_refl).
+      psimpl. exists x0. split. easy.
+      assert (ReadyWaiting i WFPop x (invPoss i x1 WFPop)).
+      {
+        assert (snd s = snd x).
+        { unfold TInvoke in H1. now psimpl. }
+        drecs.
+        constructor.
+        {
+          constructor.
+          constructor; cbn;
+          unfold wfs_idle, eval_stack_und, memSt, casSt in *;
+          auto; try now setoid_rewrite <- H.
+        }
+        {
+          constructor; cbn;
+          now rewrite eqb_id.
+        }
+      }
+      {
+        apply ready_waiting_stable.
+        psplit. exact H. easy.
+      }
+    }
+
+    cut (
+      forall P,
+      P ==> (fun _ _ => LiftSPrec (ReadyWaiting i WFPop)) ->
+        VerifyProg i (LiftSRelt (Rely i)) (LiftSRelt (Guar i))
+          P
+          wfpop
+          (fun r _ _ => LiftSPrec (ReadyDone i WFPop r))
+    ).
+    { intros. now apply H. }
+    cofix rec. intros P impH. unfold wfpop.
+
+    (* step get call *)
+    rewrite stepCall.
+    eapply SafeBind with
+      (QI:=fun _ _ => LiftSPrec (ReadyWaiting i WFPop))
+      (QR:=fun old _ _ => LiftSPrec (fun s x =>
+          match old with
+          | Some _ =>
+            ReadyWaiting i WFPop s x /\
+            exists vs, list_seg (eval_heap (memSt s)) old None vs
+          | None =>
+            ReadyDone i WFPop (PASS None) s x
+          end
+        )).
+    (* stable QI *)
+    { admit. }
+    (* stable QR *)
+    { admit. }
+    (* commit *)
+    {
+      clear rec. begin_commit.
+      psimpl. apply impH in H.
+      clear impH. psimpl.
+      unfold LiftSPrec in H. psimpl.
+      exists (eq x).
+      split; [repeat econstructor|].
+      split; [intros; subst; repeat econstructor|].
+      split.
+      {
+        exists x. split; auto.
+        destruct H7, wait_ready0, ready_inv0.
+        constructor; [repeat constructor|auto].
+        - inversion H2; subst.
+          now forward_istep_cas_aux s t.
+        - admit.
+        - now setoid_rewrite <- H6.
+      }
+      {
+        exists x. split. easy. apply eq_inj in H; subst.
+        eapply StkGetCall with (i:=i).
+        constructor; [|easy].
+        constructor; cbn. easy.
+        intros. now rewrite H0.
+      }
+    }
+
+    (* step get ret *)
+    clear impH. intro old. split.
+    {
+      clear rec. begin_commit.
+      
+      inversion H2; psimpl; psimpl.
+      inversion H2; subst.
+      ddestruct H6.
+
+      destruct H9, wait_ready0, ready_inv0.
+      subst_ist s; subst_ist t; psimpl.
+      
+      destruct old.
+      (* non-empty stack *)
+      {
+        exists (eq x3).
+        psimpl. psimpl.
+        split; [repeat econstructor|].
+        split; [econstructor; split; [eauto|constructor]|].
+        split.
+        {
+          exists x3. split; auto.
+          split.
+          - constructor; [repeat constructor|auto]; auto;
+            try now subst_ist s; subst_ist t.
+          - subst_ist s; subst_ist t.
+            eexists; eauto.
+        }
+        {
+          exists x3. split. easy. apply eq_inj in H3; subst.
+          eapply StkGetRetId with (i:=i) (old:=Some a).
+          constructor.
+          - constructor; simpl; eauto.
+            now apply differ_pointwise_comm.
+          - constructor; auto.
+            subst_ist s; subst_ist t.
+            constructor.
+        }
+      }  
+      (* empty stack *)
+      {
+        destruct ready_wait0.
+        destruct x3; subst; psimpl.
+        inversion always_atomic0; psimpl.
+        inversion same_stack0; try congruence.
+        subst_ist s; psimpl.
+
+        exists (eq (
+          comRetPoss i
+            (comInvPoss i
+              (MkPoss T (F A) VF (WFSsIdle []) PCalls PRets)
+              WFPop
+              (WFSsPend i [] WFPop)
+            )
+            WFPop
+            (WFSsIdle [])
+            (PASS None)
+        )).
+        split; [repeat econstructor|].
+        split; [econstructor; split; [now eauto|]|split].
+        (* poss step *)
+        {
+          subst.
+          (* commit call *)
+          eapply PossStepsStep with (i := i) (σ := (comInvPoss i
+            (MkPoss T (F A) VF (WFSsIdle []) PCalls PRets)
+            WFPop
+            (WFSsPend i [] WFPop)
+          )); psimpl; auto.
+          {
+            eapply PCommitCall with (m := WFPop); psimpl; auto;
+            [constructor|now rewrite eqb_id].
+          }
+          {
+            intros; rewrite eqb_nid; auto.
+          }
+          (* commit ret *)
+          eapply PossStepsStep with (i := i);
+          [| | |apply PossStepsRefl];
+          psimpl; auto.
+          {
+            eapply PCommitRet with (m := WFPop) (v := PASS None);
+            psimpl; auto; try now rewrite eqb_id.
+            constructor.
+          }
+          {
+            intros; rewrite eqb_nid; auto.
+          }
+        }
+        (* post condition *)
+        {
+          eexists; split; eauto.
+          constructor; constructor; [constructor| |]; psimpl;
+          try now rewrite eqb_id.
+          - subst_ist s; subst_ist t; psimpl; auto.
+          - unfold wfs_idle in *; psimpl; eauto.
+          - subst_ist s; subst_ist t; auto.
+        }
+        (* guarantee *)
+        {
+          exists (comRetPoss i
+          (comInvPoss i (MkPoss T (F A) VF (WFSsIdle []) PCalls PRets) WFPop
+             (WFSsPend i [] WFPop)) WFPop (WFSsIdle []) (PASS None)).
+          split. easy. apply eq_inj in H5; subst.
+          (* inversion H6; subst; clear H6. *)
+          eapply StkGetRetEmp with (i:=i).
+          constructor.
+          - constructor; simpl; eauto.
+            now apply differ_pointwise_comm.
+          - constructor; psimpl; auto.
+            subst_ist s; subst_ist t; auto.
+          - eapply VStep with (y:=comInvPoss i
+            (MkPoss T (F A) VF (WFSsIdle []) PCalls PRets)
+            WFPop
+            (WFSsPend i [] WFPop)); psimpl; auto;
+              [
+                constructor; psimpl; auto;
+                [constructor|now rewrite eqb_id]|
+                apply differ_pointwise_trivial|
+                unfold differ_pointwise; auto|
+              ].
+            eapply VStep; [| | |apply VRefl];
+            psimpl; auto;
+            try apply differ_pointwise_trivial;
+            try (unfold differ_pointwise; auto).
+            constructor; psimpl; auto;
+            try now rewrite eqb_id.
+            constructor.
+        }
+      }
+    }
+
+    destruct old as [old |].
+    (* handle empty stack return case first *)
+    2:{
+      apply SafeReturn.
+      unfold sub, subRelt.
+      intros. unfold LiftSPrec in H.
+      psimpl. exists x3. now destruct H2.
+    }
+
+    (* step read call *)
+    rewrite stepCall.
+    eapply SafeBind with
+      (QI:=fun _ _ => LiftSPrec (fun s x =>
+          ReadyWaiting i WFPop s x /\
+          exists vs, list_seg (eval_heap (memSt s)) (Some old) None vs))
+      (QR:=fun r _ _ => LiftSPrec (fun s x =>
+          match r with (v, next) =>
+          ReadyWaiting i WFPop s x /\
+          (exists h, (eval_heap (memSt s)) = Some h /\ h old = Some (v, next)) /\
+          exists vs, list_seg (eval_heap (memSt s)) (Some old) None (v :: vs)
+          end
+        )).
+    (* QI stable *)
+    { admit. }
+    (* QR stable *)
+    { admit. }
+    (* commit *)
+    {
+      clear rec. begin_commit.
+      do 2 psimpl.
+      destruct H5 as [Hready Hwait];
+      destruct Hready as [Hinv]; destruct Hinv.
+
+      exists (eq x5).
+      split; [repeat econstructor|].
+      split; [intros; subst; repeat econstructor|].
+      split.
+      {
+        inversion H2; subst; subst_ist s; subst_ist t;
+        psimpl; [|inversion same_stack0; congruence].
+        exists x5. split; auto.
+        split; eauto.
+        constructor; [do 2 constructor|auto];
+        try now subst_ist s; subst_ist t.
+      }
+      {
+        exists x5. split. easy. apply eq_inj in H5; subst.
+        eapply StkReadCall with (i:=i) (addr:=old).
+        constructor; [|easy].
+        constructor; cbn. easy.
+        intros. now rewrite H0.
+      }
+    }
+
+    (* step read ret *)
+    intros [v next]. split.
+    {
+      clear rec. begin_commit. psimpl. psimpl.
+      destruct H4, wait_ready0, ready_inv0.
+
+      exists (eq x4).
+      split; [repeat econstructor|].
+      split; [intros; subst; repeat econstructor|].
+      split.
+      {
+        inversion H2; subst; forward_istep_mem_aux s t.
+        (* old must be non-empty *)
+        2:{
+          exfalso.
+          inversion H5; subst.
+          congruence.
+        }
+        exists x4; split; auto.
+        split.
+        {
+          constructor; [do 2 constructor|auto];
+          try now subst_ist s; subst_ist t.
+        }
+        {
+          ddestruct H15.
+          inversion H5; subst.
+          inversion H14; subst h0.
+          inversion H12; subst l.
+          rewrite H13 in H15; inversion H15; subst.
+          eauto.
+        }
+      }
+      {
+        exists x4. split. easy. apply eq_inj in H4; subst.
+        eapply StkReadRet with (i:=i) (addr:=old) (v:=(v, next)).
+        - inversion H5; subst.
+          inversion H4; subst.
+          unfold location_allocated.
+          subst_ist s.
+          eexists; split; eauto.
+          congruence.
+        - constructor; [|easy].
+          constructor; cbn. easy.
+          intros. now rewrite H0.
+      }
+    }
+
+    (* step cas call *)
+    rewrite stepCall.
+    eapply SafeBind with
+      (QI:=fun _ _ => LiftSPrec (fun s x =>
+          ReadyWaiting i WFPop s x /\
+          (exists h, (eval_heap (memSt s)) = Some h /\ h old = Some (v, next)) /\
+          exists vs, list_seg (eval_heap (memSt s)) (Some old) None (v :: vs)
+        ))
+      (QR:=fun b _ _ => LiftSPrec (fun s x =>
+          if b : bool
+          then ReadyDone i WFPop (PASS (Some v)) s x
+          else ReadyDone i WFPop FAIL s x
+        )).
+    (* QI stable *)
+    { admit. }
+    (* QR stable *)
+    { admit. }
+    (* commit *)
+    {
+      clear rec. begin_commit.
+      do 2 psimpl.
+      destruct H5 as [Hready Hwait];
+      destruct Hready as [Hinv]; destruct Hinv.
+
+      exists (eq x6).
+      split; [repeat econstructor|].
+      split; [intros; subst; repeat econstructor|].
+      split.
+      {
+        inversion H2; subst; subst_ist s; subst_ist t.
+        exists x6. split; auto.
+        split; eauto.
+        constructor; [do 2 constructor|auto];
+        try now subst_ist s; subst_ist t.
+      }
+      {
+        exists x6. split. easy. apply eq_inj in H5; subst.
+        eapply StkCASCall with (i:=i) (old:=Some old) (new:=next).
+        constructor; [|easy].
+        constructor; cbn. easy.
+        intros. now rewrite H0.
+      }
+    }
+    
+    split.
+    {
+      clear rec. begin_commit.
+      psimpl.
+      destruct H4, wait_ready0, ready_inv0.
+      destruct always_atomic0 as [vs0 ?].
+      destruct x4; simpl in *.
+      destruct ready_wait0.
+      psimpl. psimpl.
+      inversion H2; subst; forward_istep_cas_aux s t;
+      ddestruct H24; psimpl.
+      (* cas succ *)
+      {
+        rename x5 into vs.
+        assert (vs0 = v :: vs) by (eapply ListSegUnique; eauto); subst.
+
+        exists (eq (
+          comRetPoss i
+            (comInvPoss i
+              (MkPoss T (F A) VF (WFSsIdle (v :: vs)) PCalls PRets)
+              WFPop
+              (WFSsPend i (v :: vs) WFPop)
+            )
+            WFPop
+            (WFSsIdle vs)
+            (PASS (Some v))
+        )).
+        split; [repeat econstructor|].
+        split; [econstructor; split; [now eauto|]|split].
+        (* poss step *)
+        {
+          subst.
+          (* commit call *)
+          eapply PossStepsStep with (i := i) (σ := (comInvPoss i
+            (MkPoss T (F A) VF (WFSsIdle (v :: vs)) PCalls PRets)
+            WFPop
+            (WFSsPend i (v :: vs) WFPop)
+          )); psimpl; auto.
+          {
+            eapply PCommitCall with (m := WFPop); psimpl; auto;
+            [constructor|now rewrite eqb_id].
+          }
+          {
+            intros; rewrite eqb_nid; auto.
+          }
+          (* commit ret *)
+          eapply PossStepsStep with (i := i);
+          [| | |apply PossStepsRefl];
+          psimpl; auto.
+          {
+            eapply PCommitRet with (m := WFPop) (v := PASS (Some v));
+            psimpl; auto; try now rewrite eqb_id.
+            constructor.
+          }
+          {
+            intros; rewrite eqb_nid; auto.
+          }
+        }
+        (* post condition *)
+        {
+          eexists; split; eauto.
+          constructor; constructor; [constructor| |]; psimpl;
+          try now rewrite eqb_id.
+          - inversion same_stack0; subst.
+            subst_ist s; subst_ist t; psimpl; auto.
+            inversion H21; subst l.
+            rewrite H5 in H22; inversion H22; subst x6.
+            rewrite H7 in H26; inversion H26; subst l2.
+            auto.
+          - unfold wfs_idle in *; psimpl; eauto.
+          - subst_ist s; subst_ist t; auto.
+        }
+        (* guarantee *)
+        {
+          exists (
+            comRetPoss i
+              (comInvPoss i
+                (MkPoss T (F A) VF (WFSsIdle (v :: vs)) PCalls PRets)
+                WFPop
+                (WFSsPend i (v :: vs) WFPop)
+              )
+              WFPop
+              (WFSsIdle vs)
+              (PASS (Some v))
+          ).
+          split. easy. apply eq_inj in H17; subst.
+          (* inversion H6; subst; clear H6. *)
+          eapply StkCASRetPopPass with (i:=i) (v:=v) (new:=next) (old:=old); eauto.
+          constructor.
+          - constructor; simpl; eauto.
+            now apply differ_pointwise_comm.
+          - constructor; psimpl; auto.
+            subst_ist s; subst_ist t; auto.
+          - eapply VStep with (y:=(comInvPoss i
+              (MkPoss T (F A) VF (WFSsIdle (v :: vs)) PCalls PRets)
+              WFPop
+              (WFSsPend i (v :: vs) WFPop)
+            )); psimpl; auto;
+              [
+                constructor; psimpl; auto;
+                [constructor|now rewrite eqb_id]|
+                apply differ_pointwise_trivial|
+                unfold differ_pointwise; auto|
+              ].
+            eapply VStep; [| | |apply VRefl];
+            psimpl; auto;
+            try apply differ_pointwise_trivial;
+            try (unfold differ_pointwise; auto).
+            constructor; psimpl; auto;
+            try now rewrite eqb_id.
+            constructor.
+        }
+      }
+      (* cas fail *)
+      {
+        exists (eq (
+          comRetPoss i
+            (comInvPoss i
+              (MkPoss T (F A) VF (WFSsIdle vs0) PCalls PRets)
+              WFPop
+              (WFSsPend i vs0 WFPop)
+            )
+            WFPop
+            (WFSsIdle vs0)
+            FAIL
+        )).
+        split; [repeat econstructor|].
+        split; [econstructor; split; [now eauto|]|split].
+        (* poss step *)
+        {
+          subst.
+          (* commit call *)
+          eapply PossStepsStep with (i := i) (σ := (comInvPoss i
+            (MkPoss T (F A) VF (WFSsIdle vs0) PCalls PRets)
+            WFPop
+            (WFSsPend i vs0 WFPop)
+          )); psimpl; auto.
+          {
+            eapply PCommitCall with (m := WFPop); psimpl; auto;
+            [constructor|now rewrite eqb_id].
+          }
+          {
+            intros; rewrite eqb_nid; auto.
+          }
+          (* commit ret *)
+          eapply PossStepsStep with (i := i);
+          [| | |apply PossStepsRefl];
+          psimpl; auto.
+          {
+            eapply PCommitRet with (m := WFPop) (v := FAIL);
+            psimpl; auto; try now rewrite eqb_id.
+            constructor.
+          }
+          {
+            intros; rewrite eqb_nid; auto.
+          }
+        }
+        (* post condition *)
+        {
+          eexists; split; eauto.
+          constructor; constructor; [constructor| |]; psimpl;
+          try (now rewrite eqb_id);
+          subst_ist s; subst_ist t; psimpl; auto.
+          unfold wfs_idle in *; psimpl; eauto.
+        }
+        (* guarantee *)
+        {
+          exists (comRetPoss i
+            (comInvPoss i
+              (MkPoss T (F A) VF (WFSsIdle vs0) PCalls PRets)
+              WFPop
+              (WFSsPend i vs0 WFPop)
+            )
+            WFPop
+            (WFSsIdle vs0)
+            FAIL).
+          split. easy. apply eq_inj in H17; subst.
+          (* inversion H6; subst; clear H6. *)
+          eapply StkCASRetPopFail with (i:=i) (new:=next) (old:=Some old); eauto.
+          constructor.
+          - constructor; simpl; eauto.
+            now apply differ_pointwise_comm.
+          - constructor; psimpl; auto.
+            subst_ist s; subst_ist t; auto.
+          - eapply VStep with (y:=comInvPoss i
+              (MkPoss T (F A) VF (WFSsIdle vs0) PCalls PRets)
+              WFPop
+              (WFSsPend i vs0 WFPop)); psimpl; auto;
+              [
+                constructor; psimpl; auto;
+                [constructor|now rewrite eqb_id]|
+                apply differ_pointwise_trivial|
+                unfold differ_pointwise; auto|
+              ].
+            eapply VStep; [| | |apply VRefl];
+            psimpl; auto;
+            try apply differ_pointwise_trivial;
+            try (unfold differ_pointwise; auto).
+            constructor; psimpl; auto;
+            try now rewrite eqb_id.
+            constructor.
+        }
+      }
+    }
+    
+    (* ret *)
+    destruct v0;
+    apply SafeReturn;
+    unfold sub, subRelt;
+    intros; unfold LiftSPrec in H;
+    psimpl; exists x4; now destruct H3.
+  Admitted.
 
   Theorem WFStackCorrect:
     VerifyImpl VE VF
@@ -599,82 +2305,188 @@ Module AtomicWFStackProof.
     (fun i _ m r _ _ => LiftSPrec (ReadyDone i m r))
     (TReturn (WFStack A)).
   Proof.
-    constructor.
-    7:{
-    Set Printing All.
+    constructor;
+    [
+      apply RelyReflexive|
+      apply RelyClosed|
+      apply GuarInRely|
+      apply InvokeInRely|
+      apply ReturnInRely|
+      apply InitialReady|
+      apply ReadyStable|
+      | |
+    ].
+    {
+      unfold sub, subPrec.
+      unfold LiftSRelt, LiftSPrec.
+      intros. psimpl.
+      assert (exists x, ρ = eq x).
+      {
+        eapply Return_pres_single.
+        exact H0.
+      }
+      psimpl.
+      eexists. split. easy.
+      unfold TReturn, InterOStep in H0.
+      psimpl. ddestruct H0. cbn in *.
+      ddestruct H0. apply sing_elem in H5.
+      psimpl. unfold mapRetPoss in H5. psimpl.
+      destruct H2, done_ready0, ready_inv0.
+      constructor; constructor.
+      {
+        unfold eval_stack_und, memSt, casSt in *.
+        setoid_rewrite <- H4.
+        setoid_rewrite H10.
+        easy.
+      }
+      {
+        unfold wfs_idle in *.
+        now setoid_rewrite H10.
+      }
+      {
+        intros.
+        unfold eval_stack_und, memSt, casSt in *.
+        setoid_rewrite <- H4 in H2. 
+        eapply write_excl0; eauto.
+      }
+    }
+    {
+      intros. destruct m.
+      {
+        eapply weakenPost.
+        apply PushCorrect.
+        {
+          unfold sub, subRelt, LiftSPrec.
+          intros. psimpl. eexists. split. easy.
+          destruct v0; easy.
+        }
+      }
+      {
+        eapply weakenPost.
+        apply PopCorrect.
+        {
+          unfold sub, subRelt, LiftSPrec.
+          intros. psimpl. eexists. easy.
+        }
+      }
+    }
+    {
+      unfold ReturnStep, LiftSPrec.
+      intros. psimpl. exists (eq x1).
+      split. do 2 econstructor.
+      split. intros. subst.
+      do 3 econstructor.
+      split.
+      {
+        intros. subst. destruct H2.
+        now destruct ready_done0.
+      }
+      split.
+      {
+        unfold TReturn.
+        split.
+        {
+          unfold Returned.
+          intros. subst. destruct H2.
+          now destruct ready_done0.
+        }
+        split.
+        {
+          split; cbn.
+          {
+            rewrite H0, eqb_id.
+            now constructor.
+          }
+          { intros. now rewrite eqb_nid. }
+        }
+        easy.
+      }
+      {
+        unfold LiftSRelt.
+        intros. apply eq_inj in H; subst.
+        exists (retPoss i x0).
+        split.
+        {
+          set_ext y.
+          unfold mapRetPoss, retPoss.
+          split; intros; psimpl.
+          {
+            destruct y, x1. cbn in *.
+            f_equal.
+            { easy. }
+            {
+              extensionality j.
+              dec_eq_nats i j.
+              now rewrite eqb_id.
+              now rewrite eqb_nid, H7.
+            }
+            {
+              extensionality j.
+              dec_eq_nats i j.
+              now rewrite eqb_id.
+              now rewrite eqb_nid, H8.
+            }
+          }
+          {
+            exists x0. cbn.
+            rewrite eqb_id. destruct H2, ready_done0.
+            repeat split; (easy || apply differ_pointwise_trivial).
+          }
+        }
+        {
+          apply StkReturn.
+          exists _, m, v.
+          {
+            unfold TReturn.
+            split.
+            {
+              unfold Returned.
+              intros. subst. destruct H2.
+              now destruct ready_done0.
+            }
+            split.
+            {
+              split; cbn.
+              {
+                rewrite H0, eqb_id.
+                now constructor.
+              }
+              { intros. now rewrite eqb_nid. }
+            }
+            split.
+            { easy. }
+            {
+              set_ext y.
+              unfold mapRetPoss, retPoss.
+              split; intros; psimpl.
+              {
+                exists x0. cbn.
+                rewrite eqb_id. destruct H2, ready_done0.
+                repeat split; (easy || apply differ_pointwise_trivial).
+              }
+              {
+                destruct y, x1. cbn in *.
+                f_equal.
+                { easy. }
+                {
+                  extensionality j.
+                  dec_eq_nats i j.
+                  now rewrite eqb_id.
+                  now rewrite eqb_nid, H7.
+                }
+                {
+                  extensionality j.
+                  dec_eq_nats i j.
+                  now rewrite eqb_id.
+                  now rewrite eqb_nid, H8.
+                }
+              }
+            }
+          }
+        }
+      }
+    }
   Qed.
 End AtomicWFStackProof.
 
 
-
-
-
-Record Complete {T A} (i : Name T) (v : option A)
-  (s : InterState (F A) (VE T A)) (x : Poss (VF T A))
-:= {
-  comp_inv : Inv s x;
-  comp_pres : contains (i, v) (pendSet s);
-  comp_emp : doneSet s = {}
-}.
-
-Record ReadyWaiting {T A} (i : Name T) {R} (m : F A R)
-  (s : InterState (F A) (VE T A)) (x : Poss (VF T A))
-:= {
-  wait_ready : Ready i s x;
-  ready_wait : Waiting i m x
-}.
-
-Record ReadyDone {T A} (i : Name T) {R} (m : F A R) (r : R)
-  (s : InterState (F A) (VE T A)) (x : Poss (VF T A))
-:= {
-  done_ready : Ready i s x;
-  ready_done : Done i m r x;
-}.
-
-From Equations Require Import Equations.
-
-Equations rde_prop {T A R}
-  (s : InterState (F A) (VE T A))
-  (i : Name T) (m : F A R) (r : R) : Prop :=
-rde_prop s i (Push v) _ :=
-  exists j, exchSt s = ExchDef {j => None} {i => Some v};
-rde_prop s i Pop v :=
-  exists j, exchSt s = ExchDef {j => v} {i => None}.
-
-Record ReadyDoneExch {T A} (i : Name T) {R} (m : F A R) (r : R)
-  (s : InterState (F A) (VE T A)) (x : Poss (VF T A))
-:= {
-  dexch_ready : ReadyDone i m r s x;
-  ready_proper : rde_prop s i m r
-}.
-
-Record Conflicted {T A} (i : Name T) {R} (m : F A R)
-  (s : InterState (F A) (VE T A)) (x : Poss (VF T A))
-:= {
-  wexch_ready : ReadyWaiting i m s x;
-  ready_improper :
-    match m with
-    | Push v => exists j w, exchSt s = ExchDef {j => Some w} {i => Some v}
-    | Pop => exists j, exchSt s = ExchDef {j => None} {i => None}
-    end
-}.
-
-
-Theorem EBStackCorrect T A :
-  VerifyImpl (VE T A) (VF T A)
-  (fun i => LiftSRelt (Rely i))
-  (fun i => LiftSRelt (Guar i))
-  (fun i _ _ => LiftSPrec (Ready i))
-  (EBStack A)
-  (fun i _ m r _ _ => LiftSPrec (ReadyDone i m r))
-  (TReturn (EBStack A)).
-Proof.
-Qed.
-
-Require Import LHL.Core.Linearizability.
-
-Theorem EBStackLin T A :
-  Lin (overObj (VE T A :> EBStack A)) (VF T A).
-eapply soundness.
-apply EBStackCorrect.
-Qed.
