Util/Heap.v
@@ -1,6 +1,24 @@
+Require Import Coq.Arith.PeanoNat.
+
 Definition Addr := nat.
 
 Definition Heap {V : Type} : Type := Addr -> option V.
 Definition heap_update {V : Type} (addr : Addr) (val : V) (h : Heap) : Heap :=
   fun addr' => if Nat.eqb addr addr' then Some val else h addr'.
 Definition empty_heap {V : Type} : Heap := fun _ => @None V.
+
+Lemma HeapUpdateOther {V : Type} (l1 l2: Addr) (val : V) (h : Heap):
+  l1 <> l2 -> heap_update l1 val h l2 = h l2.
+Proof.
+  unfold heap_update. intros.
+  destruct (Nat.eqb l1 l2) eqn:eq; auto.
+  apply Nat.eqb_eq in eq. congruence.
+Qed.
+
+Lemma HeapUpdateSelf {V : Type} (l: Addr) (val : V) (h : Heap):
+  heap_update l val h l = Some val.
+Proof.
+  unfold heap_update.
+  now rewrite Nat.eqb_refl.
+Qed.
+
